RS_Next

ironfleet/ravana/DistributedSystem.i.dfy
@@ -9,8 +9,9 @@ module DistributedSystem_i {
 
   predicate RS_Init(rs: RState, config: Config)
   {
-       LEnvironment_Init(rs.env)
+       LEnvironment_Init(rs.environment)
 
+    && config.node_logger == rs.endpoint_logger
     && NodeInit_Logger(rs.server_logger, config)
 
     && SeqIsUnique([config.node_logger] + config.node_controllers + config.node_switches)
@@ -32,4 +33,60 @@ module DistributedSystem_i {
        )
 
   }
+
+  predicate RS_Next(rs: RState, rs': RState)
+  {
+    LEnvironment_Next(rs.environment, rs'.environment) &&
+    rs.endpoint_logger == rs'.endpoint_logger &&
+    (if rs.environment.nextStep.LEnvStepHostIos? then
+        (if rs.environment.nextStep.actor == rs.endpoint_logger then
+            RS_NextOneServer_Logger(rs, rs',
+                rs.environment.nextStep.actor, rs.environment.nextStep.ios) &&
+            rs.server_controllers == rs'.server_controllers &&
+            rs.server_switches == rs'.server_switches
+        else if rs.environment.nextStep.actor in rs.server_controllers then
+            RS_NextOneServer_Controller(rs, rs',
+                rs.environment.nextStep.actor, rs.environment.nextStep.ios) &&
+            rs.server_logger == rs'.server_logger &&
+            rs.server_switches == rs'.server_switches
+        else if rs.environment.nextStep.actor in rs.server_switches then
+            RS_NextOneServer_Switch(rs, rs',
+                rs.environment.nextStep.actor, rs.environment.nextStep.ios) &&
+            rs.server_logger == rs'.server_logger &&
+            rs.server_controllers == rs'.server_controllers
+        else
+            rs.server_logger == rs'.server_logger &&
+            rs.server_controllers == rs'.server_controllers &&
+            rs.server_switches == rs'.server_switches
+        )
+      else
+        rs.server_logger == rs'.server_logger &&
+        rs.server_controllers == rs'.server_controllers &&
+        rs.server_switches == rs'.server_switches
+    )
+  }
+
+  predicate RS_NextOneServer_Logger(rs: RState, rs': RState, id: EndPoint, ios: seq<RavanaIo>)
+  requires id == rs.endpoint_logger
+  {
+        id == rs'.endpoint_logger
+     && NodeNext_Logger(rs.server_logger, rs'.server_logger, ios)
+  }
+
+  predicate RS_NextOneServer_Controller(rs: RState, rs': RState, id: EndPoint, ios: seq<RavanaIo>)
+  requires id in rs.server_controllers
+  {
+        id in rs'.server_controllers
+     && NodeNext_Controller(rs.server_controllers[id], rs'.server_controllers[id], ios)
+     && rs'.server_controllers == rs.server_controllers[id := rs'.server_controllers[id]]
+  }
+
+  predicate RS_NextOneServer_Switch(rs: RState, rs': RState, id: EndPoint, ios: seq<RavanaIo>)
+  requires id in rs.server_switches
+  {
+        id in rs'.server_switches
+     && NodeNext_Switch(rs.server_switches[id], rs'.server_switches[id], ios)
+     && rs'.server_switches == rs.server_switches[id := rs'.server_switches[id]]
+  }
+
 }
